HouLean/OpenCL/Data/ArgList.lean
@@ -1,0 +1,51 @@
+import HouLean.OpenCL.Basic
+
+namespace HouLean.OpenCL
+
+-- list with compile time support that will translate all elements to just a comma separated expression
+inductive ArgList (α : Type u) where
+  | nil : ArgList α
+  | cons (head : α) (tail : ArgList α) : ArgList α
+deriving Inhabited, BEq
+
+@[opencl_csimp]
+def ArgList.ofList (as : List α) : ArgList α :=
+  match as with
+  | [] => ArgList.nil
+  | a :: as => ArgList.cons a (.ofList as)
+
+@[opencl_csimp]
+def ArgList.ofFn (f : Fin n → α) : ArgList α :=
+  go n ⟨0, sorry_proof⟩ ArgList.nil
+where
+  @[opencl_csimp]
+  go (fuel : Nat) (i : Fin n) (xs : ArgList α) : ArgList α :=
+    match fuel with
+    | 0 => xs
+    | fuel+1 =>
+      let x := f i
+      .cons x (go fuel ⟨i.1+1, sorry_proof⟩ xs)
+
+@[opencl_csimp]def ArgList.size (xs : ArgList α) : Nat :=
+  match xs with
+  | .nil => 0
+  | .cons _ xs => xs.size + 1
+
+
+@[opencl_csimp high]
+theorem argList_one (x : α) :
+  ArgList.cons (α:=α) x ArgList.nil = (oclFunction (α → ArgList α) "" (.infix 0)) x := sorry_proof
+
+
+@[opencl_csimp]
+theorem argList_cons (x : α) (xs : ArgList α):
+  ArgList.cons (α:=α) x xs
+  =
+  (oclFunction (α → ArgList α → ArgList α) ", " (.infix 0)) x xs := sorry_proof
+
+
+-- @[opencl_csimp]
+-- theorem argList_cons2 (x y : α) (xs : ArgList α):
+--   ArgList.cons (α:=α) x (ArgList.cons y xs)
+--   =
+--   (oclFunction (α → ArgList α → ArgList α) ", " (.infix 0)) x (.cons y xs) := sorry_proof
