HouLean/OpenCL/Data/Vector.lean
@@ -2,6 +2,8 @@ import HouLean.Data.Vector
 import HouLean.OpenCL.Compiler.Main
 import HouLean.OpenCL.Data.Float
 import HouLean.OpenCL.Data.Fin
+import HouLean.OpenCL.Data.ArgList
+
 
 namespace HouLean.OpenCL
 
@@ -10,76 +12,20 @@ open Qq HouLean Math
 variable {α : Type} {n : Nat}
 
 -- constructor
-def vectorMk2 (x y : α) : Vector α 2 := #v[x,y]
-def vectorMk3 (x y z : α) : Vector α 3 := #v[x,y,z]
-def vectorMk4 (x y z w : α) : Vector α 4 := #v[x,y,z,w]
-def vectorMk8 (x0 x1 x2 x3 x4 x5 x6 x7 : α) : Vector α 8 :=
-  #v[x0, x1, x2, x3, x4, x5, x6, x7]
-def vectorMk16 (x0 x1 x2 x3 x4 x5 x6 x7 x8 x9 x10 x11 x12 x13 x14 x15 : α) : Vector α 16 :=
-  #v[x0,x1,x2,x3,x4,x5,x6,x7,x8,x9,x10,x11,x12,x13,x14,x15]
-
-
-implemented_by (x y : α) : #v[x,y] = vectorMk2 x y
-implemented_by (x y z : α) : #v[x,y,z] = vectorMk3 x y z := by rfl
-implemented_by (x y z w : α) : #v[x,y,z,w] = vectorMk4 x y z w := by rfl
-implemented_by (x0 x1 x2 x3 x4 x5 x6 x7 : α) :
-   #v[x0, x1, x2, x3, x4, x5, x6, x7] = (vectorMk8 x0 x1 x2 x3 x4 x5 x6 x7) := by rfl
-implemented_by (x0 x1 x2 x3 x4 x5 x6 x7 x8 x9 x10 x11 x12 x13 x14 x15 : α) :
-  #v[x0,x1,x2,x3,x4,x5,x6,x7,x8,x9,x10,x11,x12,x13,x14,x15]
+implemented_by [t : AtomicOpenCLType α] [Inhabited α] (n) (xs : List α) (h) :
+  Vector.mk (n:=n) xs.toArray h
   =
-  (vectorMk16 x0 x1 x2 x3 x4 x5 x6 x7 x8 x9 x10 x11 x12 x13 x14 x15) := by rfl
+  (oclFunction (ArgList α → Vector α n) s!"({t.name}{n})" .constructor)
+  (ArgList.ofList xs)
 
-section
-variable [AtomicOpenCLType α]
+-- ofFn
+implemented_by [t : AtomicOpenCLType α] [Inhabited α] (n) (f : (Fin n) → α) :
+  Vector.ofFn f
+  =
+  (oclFunction (ArgList α → Vector α n) s!"({t.name}{n})" .constructor)
+  (ArgList.ofFn f)
 
-instance : OpenCLFunction (vectorMk2 (α:=α)) where
-  name :=
-    let t : OpenCLType (Vector α 2) := by infer_instance
-    s!"({t.name})"
-  kind := .constructor
-
-instance : OpenCLFunction (vectorMk3 (α:=α)) where
-  name :=
-    let t : OpenCLType (Vector α 3) := by infer_instance
-    s!"({t.name})"
-  kind := .constructor
-
-instance : OpenCLFunction (vectorMk4 (α:=α)) where
-  name :=
-    let t : OpenCLType (Vector α 4) := by infer_instance
-    s!"({t.name})"
-  kind := .constructor
-
-instance : OpenCLFunction (vectorMk8 (α:=α)) where
-  name :=
-    let t : OpenCLType (Vector α 8) := by infer_instance
-    s!"({t.name})"
-  kind := .constructor
-
-instance : OpenCLFunction (vectorMk16 (α:=α)) where
-  name :=
-    let t : OpenCLType (Vector α 16) := by infer_instance
-    s!"({t.name})"
-  kind := .constructor
-
-
--- projections and element access
-instance : OpenCLFunction (@Vector.x α n) where
-  name := ".x"
-  kind := .postfix
-
-instance : OpenCLFunction (@Vector.y α n) where
-  name := ".y"
-  kind := .postfix
-
-instance : OpenCLFunction (@Vector.z α n) where
-  name := ".z"
-  kind := .postfix
-
-instance : OpenCLFunction (@Vector.w α n) where
-  name := ".w"
-  kind := .postfix
-end
+attribute [opencl_csimp] inlinedLoop inlinedLoop.go
 
 def componentProjection (i : Nat) : String :=
      (if i = 0 then
@@ -117,122 +63,23 @@ theorem opencl_rewrite_vector_getElem_nat [Inhabited α] (v : Vector α n) (i : 
 theorem Vector.getElemFin_eq_getElemNat' (v : Vector α n) (i : Fin m) (h) :
   v[i]'h = v[i.1] := by rfl
 
--- ofFn
-implemented_by (f : (Fin 2) → α) : Vector.ofFn f = #v[f 0, f 1]
-implemented_by (f : (Fin 3) → α) : Vector.ofFn f = #v[f 0, f 1, f 2]
-implemented_by (f : (Fin 4) → α) : Vector.ofFn f = #v[f 0, f 1, f 2, f 3]
-implemented_by (f : (Fin 8) → α) : Vector.ofFn f = #v[f 0, f 1, f 2, f 3, f 4, f 5, f 6, f 7]
-implemented_by (f : (Fin 16) → α) : Vector.ofFn f =
-  #v[f 0, f 1, f 2, f 3, f 4, f 5, f 6, f 7,
-     f 8, f 9, f 10, f 11, f 12, f 13, f 14, f 15]
-
 -- map
-section Map
-variable {β} (f : α → β)
-implemented_by (v : Vector α 2) : v.map f = #v[f v.x, f v.y]
-implemented_by (v : Vector α 3) : v.map f = #v[f v.x, f v.y, f v.z]
-implemented_by (v : Vector α 4) : v.map f = #v[f v.x, f v.y, f v.z, f v.w]
-implemented_by (v : Vector α 8) :
-    v.map f = #v[f v[0],f v[1],f v[2],f v[3],
-                 f v[4],f v[5],f v[6],f v[7]]
-implemented_by (v : Vector α 16) :
-    v.map f = #v[f v[0],f v[1],f v[2],f v[3],
-                 f v[4],f v[5],f v[6],f v[7],
-                 f v[8],f v[9],f v[10],f v[11],
-                 f v[12],f v[13],f v[14],f v[15]]
-end Map
+implemented_by {β} (f : α → β) (v : Vector α n) :
+    v.map f = let v := v; .ofFn (fun i => f (v[i]))
+implemented_by {β} (f : Nat → α → β) (v : Vector α n) :
+    v.mapIdx f = let v := v; .ofFn (fun i => f i.1 (v[i]))
+implemented_by {β} (f : (i : Nat) → α → i < n → β) (v : Vector α n) :
+    v.mapFinIdx f = let v := v; .ofFn (fun i => f i.1 (v[i]) (by grind))
 
-section MapIdx
-variable {β} (f : Nat → α → β)
-implemented_by (v : Vector α 2) : v.mapIdx f = #v[f 0 v.x, f 1 v.y]
-implemented_by (v : Vector α 3) : v.mapIdx f = #v[f 0 v.x, f 1 v.y, f 2 v.z]
-implemented_by (v : Vector α 4) : v.mapIdx f = #v[f 0 v.x, f 1 v.y, f 2 v.z, f 3 v.w]
-implemented_by (v : Vector α 8) :
-  v.mapIdx f
-  =
-  #v[f 0 v[0], f 1 v[1], f 2 v[2], f 3 v[3],
-     f 4 v[4], f 5 v[5], f 6 v[6], f 7 v[7]]
-implemented_by (v : Vector α 16) :
-  v.mapIdx f
-  =
-  #v[f 0 v[0], f 1 v[1], f 2 v[2], f 3 v[3],
-     f 4 v[4], f 5 v[5], f 6 v[6], f 7 v[7],
-     f 8 v[8], f 9 v[9], f 10 v[10], f 11 v[11],
-     f 12 v[12], f 13 v[13], f 14 v[14], f 15 v[15]]
-end MapIdx
+-- fold
+implemented_by {β} (f : β → α → β) (init : β) (v : Vector α n) :
+    v.foldl f init = let v := v; inlinedLoop n (fun i x => f x (v[i])) init
+implemented_by {β} (f : α → β → β) (init : β) (v : Vector α n) :
+    v.foldr f init = let v := v; inlinedLoop n (fun i x => f v[n-i-1] x) init
 
-section MapFinIdx
-variable {β}
-implemented_by (v : Vector α 2) (f : (i : Nat) → α → (h : i < 2) → β) :
-  v.mapFinIdx f
-  =
-  #v[f 0 v.x (by grind), f 1 v.y (by grind)]
+-- sum
+implemented_by [Add α] [Zero α] (u : Vector α n) : u.sum = let u := u; u.foldl (· + ·) 0
 
-implemented_by (v : Vector α 3) (f : (i : Nat) → α → (h : i < 3) → β) :
-  v.mapFinIdx f
-  =
-  #v[f 0 v.x (by grind), f 1 v.y (by grind), f 2 v.z (by grind)]
-
-implemented_by (v : Vector α 4) (f : (i : Nat) → α → (h : i < 4) → β) :
-  v.mapFinIdx f
-  =
-  #v[f 0 v.x (by grind), f 1 v.y (by grind), f 2 v.z (by grind), f 3 v.w (by grind)]
-
-end MapFinIdx
-
-
-section ZipMap
-variable (f : α×β → γ)
-implemented_by (u : Vector α 2) (v : Vector β 2) :
-    (u.zip v).map f
-    =
-    #v[f (u.x,v.x), f (u.y,v.y)] := by simp[Vector.x, Vector.y]; grind
-
-implemented_by (u : Vector α 3) (v : Vector β 3) :
-    (u.zip v).map f
-    =
-    #v[f (u.x,v.x), f (u.y,v.y), f (u.z,v.z)] := by simp[Vector.x, Vector.y, Vector.z]; grind
-
-implemented_by (u : Vector α 4) (v : Vector β 4) :
-    (u.zip v).map f
-    =
-    #v[f (u.x,v.x), f (u.y,v.y), f (u.z,v.z), f (u.w,v.w)] := by simp[Vector.x, Vector.y, Vector.z, Vector.w]; grind
-
-implemented_by (u : Vector α 8) (v : Vector β 8) :
-    (u.zip v).map f
-    =
-    #v[f (u[0],v[0]), f (u[1],v[1]), f (u[2],v[2]), f (u[3],v[3]),
-       f (u[4],v[4]), f (u[5],v[5]), f (u[6],v[6]), f (u[7],v[7])] := by sorry_proof
-
-implemented_by (u : Vector α 16) (v : Vector β 16) :
-    (u.zip v).map f
-    =
-    #v[f (u[0],v[0]), f (u[1],v[1]), f (u[2],v[2]), f (u[3],v[3]),
-       f (u[4],v[4]), f (u[5],v[5]), f (u[6],v[6]), f (u[7],v[7]),
-       f (u[8],v[8]), f (u[9],v[9]), f (u[10],v[10]), f (u[11],v[11]),
-       f (u[12],v[12]), f (u[13],v[13]), f (u[14],v[14]), f (u[15],v[15])] := sorry_proof
-end ZipMap
-
-section Foldl
-variable {β} (f : β → α → β) (init : β)
-implemented_by (u : Vector α 2) : u.foldl f init = f (f init u.x) u.y
-implemented_by (u : Vector α 3) : u.foldl f init = f (f (f init u.x) u.y) u.z
-implemented_by (u : Vector α 4) : u.foldl f init = f (f (f (f init u.x) u.y) u.z) u.w
-end Foldl
-
-
-section Foldr
-variable {β} (f : α → β → β) (init : β)
-implemented_by (u : Vector α 2) : u.foldr f init = f u.x (f u.y init)
-implemented_by (u : Vector α 3) : u.foldr f init = f u.x (f u.y (f u.z init))
-implemented_by (u : Vector α 4) : u.foldr f init = f u.x (f u.y (f u.z (f u.w init)))
-end Foldr
-
-section Sum
-variable [Add α] [Zero α]
-implemented_by (u : Vector α n) : u.sum = u.foldl (· + ·) 0
-end Sum
-
-
+-- zero
 implemented_by [Zero α] : (0 : Vector α n) = Vector.zero (α:=α) (n:=n)
 implemented_by (a : α) : Vector.replicate n a = .ofFn (fun _ => a)
